compiler/bootstrap/translation/to_patProgScript.sml
@@ -1,73 +1,10 @@
 (*
   Translate the backend phase from flatLang to patLang.
 *)
-open preamble ml_translatorLib ml_translatorTheory to_flatProgTheory
+open preamble
 
 val _ = new_theory "to_patProg";
-val _ = translation_extends "to_flatProg";
 
-val _ = ml_translatorLib.ml_prog_update (ml_progLib.open_module "to_patProg");
+(* FIXME: retire entirely *)
 
-val _ = ml_translatorLib.use_string_type true;
-
-(* ------------------------------------------------------------------------- *)
-(* Setup                                                                     *)
-(* ------------------------------------------------------------------------- *)
-
-val RW = REWRITE_RULE
-val RW1 = ONCE_REWRITE_RULE
-fun list_dest f tm =
-  let val (x,y) = f tm in list_dest f x @ list_dest f y end
-  handle HOL_ERR _ => [tm];
-val dest_fun_type = dom_rng
-val mk_fun_type = curry op -->;
-fun list_mk_fun_type [ty] = ty
-  | list_mk_fun_type (ty1::tys) =
-      mk_fun_type ty1 (list_mk_fun_type tys)
-  | list_mk_fun_type _ = fail()
-
-val _ = add_preferred_thy "-";
-val _ = add_preferred_thy "termination";
-
-val NOT_NIL_AND_LEMMA = Q.prove(
-  `(b <> [] /\ x) = if b = [] then F else x`,
-  Cases_on `b` THEN FULL_SIMP_TAC std_ss []);
-
-val extra_preprocessing = ref [MEMBER_INTRO,MAP];
-
-fun def_of_const tm = let
-  val res = dest_thy_const tm handle HOL_ERR _ =>
-              failwith ("Unable to translate: " ^ term_to_string tm)
-  val name = (#Name res)
-  fun def_from_thy thy name =
-    DB.fetch thy (name ^ "_pmatch") handle HOL_ERR _ =>
-    DB.fetch thy (name ^ "_def") handle HOL_ERR _ =>
-    DB.fetch thy (name ^ "_DEF") handle HOL_ERR _ =>
-    DB.fetch thy name
-  val def = def_from_thy "termination" name handle HOL_ERR _ =>
-            def_from_thy (#Thy res) name handle HOL_ERR _ =>
-            failwith ("Unable to find definition of " ^ name)
-  val def = def |> RW (!extra_preprocessing)
-                |> CONV_RULE (DEPTH_CONV BETA_CONV)
-                (* TODO: This ss messes up defs containing if-then-else
-                with constant branches
-                |> SIMP_RULE bool_ss [IN_INSERT,NOT_IN_EMPTY]*)
-                |> REWRITE_RULE [NOT_NIL_AND_LEMMA]
-  in def end
-
-val _ = (find_def_for_const := def_of_const);
-
-val _ = use_long_names:=true;
-
-(* ------------------------------------------------------------------------- *)
-(* flat_to_pat                                                               *)
-(* ------------------------------------------------------------------------- *)
-
-val res = translate flat_to_patTheory.compile_def;
-
-(* ------------------------------------------------------------------------- *)
-
-val () = Feedback.set_trace "TheoryPP.include_docs" 0;
-val _ = ml_translatorLib.ml_prog_update (ml_progLib.close_module NONE);
-val _ = ml_translatorLib.clean_on_exit := true;
 val _ = export_theory ();
